Completed unification!

01Unification/Substitution.thy
@@ -8,6 +8,9 @@ fun subst :: "subst \<Rightarrow> expr \<Rightarrow> expr" where
   "subst s (Var y) = (case s y of Some e \<Rightarrow> e | None \<Rightarrow> Var y)"
 | "subst s (Ctor k es) = Ctor k (map (subst s) es)"
 
+definition subst_vars :: "subst \<Rightarrow> string set" where
+  "subst_vars s = \<Union> (vars ` ran s)"
+
 fun list_subst :: "string \<Rightarrow> expr \<Rightarrow> (expr \<times> expr) list \<Rightarrow> (expr \<times> expr) list" where
   "list_subst x e' [] = []"
 | "list_subst x e' ((e\<^sub>1, e\<^sub>2) # ess) = (subst [x \<mapsto> e'] e\<^sub>1, subst [x \<mapsto> e'] e\<^sub>2) # list_subst x e' ess"
@@ -20,10 +23,10 @@ fun list_unifier :: "subst \<Rightarrow> (expr \<times> expr) list \<Rightarrow>
 | "list_unifier s ((e\<^sub>1, e\<^sub>2) # ess) = ((s unifies e\<^sub>1 and e\<^sub>2) \<and> list_unifier s ess)"
 
 definition extend_subst :: "string \<Rightarrow> expr \<Rightarrow> subst \<Rightarrow> subst" where
-  "extend_subst x e s y = (if x = y then Some e else map_option (subst [x \<mapsto> e]) (s y))"
+  "extend_subst x e s = (s(x \<mapsto> subst s e))"
 
 definition ordered_subst :: "subst \<Rightarrow> bool" where
-  "ordered_subst s = (dom s \<inter> \<Union> (vars ` ran s) = {})"
+  "ordered_subst s = (dom s \<inter> subst_vars s = {})"
 
 lemma [simp]: "x \<notin> vars e \<Longrightarrow> vars (subst [x \<mapsto> e'] e) = vars e"
   and [simp]: "x \<notin> varss es \<Longrightarrow> varss (map (subst [x \<mapsto> e']) es) = varss es"
@@ -53,18 +56,35 @@ lemma [simp]: "list_vars (list_subst x e ess) =
     list_vars ess - {x} \<union> (if x \<in> list_vars ess then vars e else {})"
   by simp
 
+lemma [simp]: "vars (subst s e) \<subseteq> vars e - dom s \<union> subst_vars s"
+  and [simp]: "varss (map (subst s) es) \<subseteq> varss es - dom s \<union> subst_vars s"
+  by (induction e and es rule: vars_varss.induct) 
+     (auto simp add: subst_vars_def ranI split: option.splits)
+
+lemma [simp]: "subst_vars Map.empty = {}"
+  by (simp add: subst_vars_def)
+
 lemma [simp]: "dom (extend_subst x e s) = insert x (dom s)"
   by (auto simp add: extend_subst_def)
 
-lemma [simp]: "x \<notin> dom s \<Longrightarrow> ran (extend_subst x e s) = insert e (subst [x \<mapsto> e] ` ran s)"
-  by (auto simp add: extend_subst_def ran_def)
+lemma [simp]: "x \<notin> dom s \<Longrightarrow> subst_vars (extend_subst x e s) = vars (subst s e) \<union> subst_vars s"
+  by (auto simp add: extend_subst_def subst_vars_def)
 
 lemma [simp]: "ordered_subst Map.empty"
   by (simp add: ordered_subst_def)
 
-lemma [simp]: "ordered_subst s \<Longrightarrow> x \<notin> vars e \<Longrightarrow> vars e \<inter> dom s = {} \<Longrightarrow> x \<notin> dom s \<Longrightarrow> 
-    ordered_subst (extend_subst x e s)"
-  by (auto simp add: ordered_subst_def split: if_splits)
+lemma [simp]: "ordered_subst s \<Longrightarrow> x \<notin> vars e \<Longrightarrow> x \<notin> dom s \<Longrightarrow> x \<notin> subst_vars s \<Longrightarrow>
+  ordered_subst (extend_subst x e s)"
+proof (unfold ordered_subst_def)
+  assume D: "dom s \<inter> subst_vars s = {}"
+  assume E: "x \<notin> vars e"
+  assume S: "x \<notin> dom s"
+  assume R: "x \<notin> subst_vars s"
+  have V: "vars (subst s e) \<subseteq> vars e - dom s \<union> subst_vars s" by simp
+  with E R have A: "x \<notin> vars (subst s e)" by blast
+  from D V have "dom s \<inter> vars (subst s e) = {}" by blast
+  with A D S R show "dom (extend_subst x e s) \<inter> subst_vars (extend_subst x e s) = {}" by auto
+qed
 
 lemma [simp]: "s unifies\<^sub>l (ess\<^sub>1 @ ess\<^sub>2) = (s unifies\<^sub>l ess\<^sub>1 \<and> s unifies\<^sub>l ess\<^sub>2)"
   by (induction s ess\<^sub>1 rule: list_unifier.induct) simp_all
@@ -76,75 +96,59 @@ proof (induction es\<^sub>1 arbitrary: es\<^sub>2)
   thus ?case by (induction es\<^sub>2) simp_all
 qed simp_all
 
-lemma unify_subst_one: "s unifies e\<^sub>1 and e\<^sub>2 \<Longrightarrow> s unifies Var x and e' \<Longrightarrow> x \<notin> vars e' \<Longrightarrow>
-    s unifies subst [x \<mapsto> e'] e\<^sub>1 and subst [x \<mapsto> e'] e\<^sub>2"
-proof (induction e\<^sub>1 arbitrary: e\<^sub>2)
-  case (Var y)
-  thus ?case 
-  proof (induction e\<^sub>2)
-    case (Ctor k\<^sub>2 es\<^sub>2)
-    thus ?case
-    proof (cases "x = y")
-      case True
-      from Ctor have "(case s y of None \<Rightarrow> Var y | Some e \<Rightarrow> e) = Ctor k\<^sub>2 (map (subst s) es\<^sub>2)" by simp
-      from Ctor have "(case s x of None \<Rightarrow> Var x | Some e \<Rightarrow> e) = subst s e'" by simp
-      from Ctor have "x \<notin> vars e'" by simp
-
-  
-      have "subst s e' = Ctor k\<^sub>2 (map (subst s \<circ> subst [x \<mapsto> e']) es\<^sub>2)" by simp
-      with True have "s unifies subst [x \<mapsto> e'] (Var y) and subst [x \<mapsto> e'] (Ctor k\<^sub>2 es\<^sub>2)" by simp
-      thus ?thesis by blast
-    next
-      case False
-      from Ctor have "(case s y of None \<Rightarrow> Var y | Some e \<Rightarrow> e) = Ctor k\<^sub>2 (map (subst s) es\<^sub>2)" by simp
-      from Ctor have "(case s x of None \<Rightarrow> Var x | Some e \<Rightarrow> e) = subst s e'" by simp
-      from Ctor have "x \<notin> vars e'" by simp
-
-  
-      have "(case s y of None \<Rightarrow> Var y | Some e \<Rightarrow> e) = Ctor k\<^sub>2 (map (subst s \<circ> subst [x \<mapsto> e']) es\<^sub>2)" by simp
-      with False have "s unifies subst [x \<mapsto> e'] (Var y) and subst [x \<mapsto> e'] (Ctor k\<^sub>2 es\<^sub>2)" by simp
-      thus ?thesis by blast
-    qed
-  qed (auto split: option.splits)
-next
-  case (Ctor k\<^sub>1 es\<^sub>1)
-  thus ?case by simp
-qed
-
-lemma [simp]: "x \<notin> vars e \<Longrightarrow> s unifies Var x and e \<Longrightarrow> s unifies\<^sub>l ess \<Longrightarrow> 
-  s unifies\<^sub>l list_subst x e ess"
-proof (induction x e ess rule: list_subst.induct)
-  case (2 x e' e\<^sub>1 e\<^sub>2 ess)
-  hence "s unifies Var x and e'" by simp
-  moreover from 2 have "s unifies e\<^sub>1 and e\<^sub>2" by simp
-  moreover from 2 have "x \<notin> vars e'" by simp
-  ultimately have "s unifies subst [x \<mapsto> e'] e\<^sub>1 and subst [x \<mapsto> e'] e\<^sub>2" by (metis unify_subst_one)
-  with 2 show ?case by simp
-qed simp_all
-
-lemma [simp]: "s x = Some e' \<Longrightarrow> x \<in> vars e \<Longrightarrow> e \<noteq> Var x \<Longrightarrow> size e' < size (subst s e)"
-  and [simp]: "s x = Some e' \<Longrightarrow> x \<in> varss es \<Longrightarrow> size e' < size_list (size \<circ> subst s) es"
+lemma occurs_check' [simp]: "x \<in> vars e \<Longrightarrow> e \<noteq> Var x \<Longrightarrow> size (subst s (Var x)) < size (subst s e)"
+  and [simp]: "x \<in> varss es \<Longrightarrow> size (subst s (Var x)) < size_list (size \<circ> subst s) es"
 proof (induction e and es rule: vars_varss.induct)
   case (4 e es)
-  then show ?case by force
+  thus ?case by force
 qed fastforce+
 
-lemma occurs_check [simp]: "x \<in> vars e \<Longrightarrow> e \<noteq> Var x \<Longrightarrow> s x = Some (subst s e) \<Longrightarrow> False"
-proof (induction "s x")
-  case (Some e')
-  from Some(1, 2, 3) have "size e' < size (subst s e)" by simp
-  with Some show ?case by simp
-qed simp_all
-
+lemma occurs_check [simp]: "x \<in> vars e \<Longrightarrow> e \<noteq> Var x \<Longrightarrow> s unifies Var x and e \<Longrightarrow> False"
+proof -
+  assume "x \<in> vars e" and "e \<noteq> Var x" 
+  hence "size (subst s (Var x)) < size (subst s e)" by (metis occurs_check')
+  moreover assume "s unifies Var x and e"
+  ultimately show ?thesis by simp
+qed
 
 lemma [simp]: "x \<in> varss es \<Longrightarrow> s x \<noteq> Some (Ctor k (map (subst s) es))"
-proof (rule)
+proof
   assume "x \<in> varss es"
   hence X: "x \<in> vars (Ctor k es)" by simp
   have Y: "Ctor k es \<noteq> Var x" by simp
   assume "s x = Some (Ctor k (map (subst s) es))"
-  hence "s x = Some (subst s (Ctor k es))" by simp
+  hence "s unifies Var x and Ctor k es" by simp
   with X Y show False by (metis occurs_check)
 qed
+
+lemma [simp]: "subst s (subst [x \<mapsto> e'] e) = subst (extend_subst x e' s) e"
+  by (induction e) (simp_all add: extend_subst_def split: option.splits)
+
+lemma [simp]: "s unifies\<^sub>l list_subst x e ess = (extend_subst x e s unifies\<^sub>l ess)"
+  by (induction s ess rule: list_unifier.induct) simp_all
+
+lemma [simp]: "extend_subst x e s x = Some (subst s e)"
+  by (simp add: extend_subst_def)
+
+lemma [simp]: "x \<notin> vars e \<Longrightarrow> subst (s(x := y)) e = subst s e"
+  and [simp]: "x \<notin> varss es \<Longrightarrow> map (subst (s(x := y))) es = map (subst s) es"
+  by (induction e and es rule: vars_varss.induct) (simp_all split: option.splits)
+
+lemma [simp]: "x \<notin> vars e \<Longrightarrow> subst (extend_subst x e' s) e = subst s e"
+  by (simp_all add: extend_subst_def)
+
+lemma [simp]: "s x = None \<Longrightarrow> subst (s(x \<mapsto> Var x)) e = subst s e"
+  by (induction e) simp_all
+
+lemma [simp]: "s x = None \<Longrightarrow> (s(x \<mapsto> Var x) unifies\<^sub>l ess) = (s unifies\<^sub>l ess)"
+  by (induction s ess rule: list_unifier.induct) simp_all
+
+lemma [simp]: "s y = Some (Var x) \<Longrightarrow> s x = None \<Longrightarrow> 
+    extend_subst x (Var y) s unifies\<^sub>l ess = (s unifies\<^sub>l ess)"
+  by (simp add: extend_subst_def)
+
+lemma var_subst [simp]: "Var x = subst s e \<Longrightarrow> 
+    (e = Var x \<and> s x = None) \<or> (\<exists>y. e = Var y \<and> s y = Some (Var x))"
+  by (induction e) (simp_all split: option.splits)
 
 end
